@prefix rdf: <http://www.w3.org/1999/02/22-rdf-syntax-ns#> .
@prefix a: <http://protege.stanford.edu/system#> .
@prefix dct: <http://purl.org/dc/terms/> .
@prefix dso: <http://purl.org/ontology/dso#> .
@prefix foaf: <http://xmlns.com/foaf/0.1/> .
@prefix geo: <http://www.w3.org/2003/01/geo/wgs84_pos#> .
@prefix gr: <http://purl.org/goodrelations/v1#> .
@prefix lso: <http://purl.org/ontology/libso#> .
@prefix org: <http://www.w3.org/ns/org#> .
@prefix owl: <http://www.w3.org/2002/07/owl#> .
@prefix rdfs: <http://www.w3.org/2000/01/rdf-schema#> .
@prefix s: <http://schema.org/> .
@prefix service: <http://purl.org/ontology/service#> .
@prefix vann: <http://purl.org/vocab/vann/> .
@prefix vcard: <http://www.w3.org/2006/vcard/ns#> .
@prefix voaf: <http://purl.org/vocommons/voaf#> .
@prefix xml: <http://www.w3.org/XML/1998/namespace> .
@prefix xsd: <http://www.w3.org/2001/XMLSchema#> .

gr:DayOfWeek
    a rdfs:Class ;
    rdfs:comment "The day of the week, used to specify to which day the opening hours of a gr:OpeningHoursSpecification refer." ;
    rdfs:isDefinedBy <http://purl.org/goodrelations/v1#> ;
    rdfs:label "Day of Week"@en .

gr:Friday
    a gr:DayOfWeek .

gr:Monday
    a gr:DayOfWeek .

gr:OpeningHoursSpecification
    a rdfs:Class ;
    rdfs:comment "This is a conceptual entity that holds together all information about the opening hours on a given day (gr:DayOfWeek)." ;
    rdfs:isDefinedBy <http://purl.org/goodrelations/v1#> ;
    rdfs:label "Opening hours specification"@en .

gr:Saturday
    a gr:DayOfWeek .

gr:Sunday
    a gr:DayOfWeek .

gr:Thursday
    a gr:DayOfWeek .

gr:Tuesday
    a gr:DayOfWeek .

gr:UnitPriceSpecification
    a rdfs:Class ;
    rdfs:comment """A unit price specification is a conceptual entity that 
        specifies the price asked for a given gr:Offering by the respective gr:Business
        Entity. An offering may be linked to multiple unit price specifications that
        specify alternative prices for non-overlapping sets of conditions (e.g. 
        quantities or sales regions) or with differing validity periods...""" ;
    rdfs:isDefinedBy <http://purl.org/goodrelations/v1#> ;
    rdfs:label "Unit price specification"@en .

gr:Wednesday
    a gr:DayOfWeek .

gr:closes
    a rdf:Property ;
    rdfs:comment "The closing hour of the gr:Location on the given gr:DayOfWeek..." ;
    rdfs:domain gr:OpeningHoursSpecification ;
    rdfs:isDefinedBy <http://purl.org/goodrelations/v1#> ;
    rdfs:label "closes (1..1)"@en ;
    rdfs:range xsd:time .

gr:hasCurrency
    a rdf:Property ;
    rdfs:comment "The currency for all prices in the gr:PriceSpecification given using the ISO 4217 standard (3 characters)." ;
    rdfs:domain gr:PriceSpecification ;
    rdfs:isDefinedBy <http://purl.org/goodrelations/v1#> ;
    rdfs:label "has currency (1..1)"@en ;
    rdfs:range xsd:string .

gr:hasCurrencyValue
    a rdf:Property ;
    rdfs:comment """This property specifies the amount of money for a price per
    unit, shipping charges, or payment charges. The currency and other relevant
    details are attached to the respective gr:PriceSpecification etc...""" ;
    rdfs:domain gr:PriceSpecification ;
    rdfs:isDefinedBy <http://purl.org/goodrelations/v1#> ;
    rdfs:label "has currency value (0..1)"@en ;
    rdfs:range xsd:float .

gr:hasOpeningHoursDayOfWeek
    a rdf:Property ;
    rdfs:comment "This specifies the gr:DayOfWeek to which the gr:OpeningHoursSpecification is related..." ;
    rdfs:domain gr:OpeningHoursSpecification ;
    rdfs:isDefinedBy <http://purl.org/goodrelations/v1#> ;
    rdfs:label "has opening hours day of week (1..*)"@en ;
    rdfs:range gr:DayOfWeek .

gr:hasOpeningHoursSpecification
    a rdf:Property ;
    rdfs:comment "For use in LSO: This property links a lso:Local to a gr:OpeningHoursSpecification.", "This property links a gr:Location to a gr:OpeningHoursSpecification." ;
    rdfs:domain gr:Location, lso:Local, s:Place ;
    rdfs:isDefinedBy <http://purl.org/goodrelations/v1#> ;
    rdfs:label "has opening hours specification (0..*)"@en ;
    rdfs:range gr:OpeingHoursSpecification .

gr:hasPriceSpecification
    a rdf:Property ;
    rdfs:comment "For use in LSO: This property links a lso:LibraryService to a gr:PriceSpecification.", "This links a gr:Offering to a gr:PriceSpecification or specifications..." ;
    rdfs:domain gr:Offering, lso:LibraryService, s:Offer ;
    rdfs:isDefinedBy <http://purl.org/goodrelations/v1#> ;
    rdfs:label "has price specification (0..*)"@en ;
    rdfs:range gr:PriceSpecification .

gr:opens
    a rdf:Property ;
    rdfs:comment "The opening hour of the gr:Location on the given gr:DayOf- Week..." ;
    rdfs:domain gr:OpeningHoursSpecification ;
    rdfs:isDefinedBy <http://purl.org/goodrelations/v1#> ;
    rdfs:label "opens (1..1)"@en ;
    rdfs:range xsd:time .

dso:Digitization
    a:role "concrete" ;
    a rdfs:Class ;
    rdfs:isDefinedBy <http://purl.org/ontology/dso> ;
    rdfs:label "Scanner"@en ;
    rdfs:subClassOf lso:CopierOrScanner .

dso:InterLoan
    a rdfs:Class ;
    rdfs:isDefinedBy <http://purl.org/ontology/dso> ;
    rdfs:label "Fernleihe"@de, "Interloan"@en ;
    rdfs:subClassOf dso:DocumentService, lso:LocalUsage .

dso:OpenAccess
    a rdfs:Class ;
    rdfs:isDefinedBy <http://purl.org/ontology/dso> ;
    rdfs:label "Open Access"@en ;
    rdfs:subClassOf dso:DocumentService, lso:WebBasedUsage .

dso:Presentation
    a rdfs:Class ;
    rdfs:comment "A service to provide space to use the media collection on site at the library, e.g. in a reading room." ;
    rdfs:isDefinedBy <http://purl.org/ontology/dso> ;
    rdfs:label "Presentation"@en, "Präsenzansicht"@de ;
    rdfs:subClassOf dso:documentService, lso:LocalUSage .

dso:loan
    a rdfs:Class ;
    rdfs:isDefinedBy <http://purl.org/ontology/dso> ;
    rdfs:label "Fernleihe"@de, "Interloan"@en ;
    rdfs:subClassOf dso:DocumentService, lso:LocalUsage .

<http://purl.org/ontology/libso>
    dct:creator "Matthias Letsch" ;
    dct:description "An Ontology to define a classification of conventional services provided by libraries." ;
    dct:modified "2013-12-09"^^xsd:date ;
    dct:title "Library [Service Ontology]"@en ;
    vann:preferredNamespacePrefix "lso" ;
    vann:preferredNamespaceUri "http://purl.org/ontology/libso#" ;
    a voaf:Vocabulary, owl:Ontology ;
    owl:versionInfo "0.1" .

lso:Catalogue
    a rdfs:Class ;
    rdfs:isDefinedBy <http://purl.org/ontology/libso> ;
    rdfs:label "Catalogue"@en, "Katalog"@de ;
    rdfs:subClassOf lso:WebBasedUsage .

lso:Condition
    a rdfs:Class ;
    rdfs:comment "Defines the terms of use for a service." ;
    rdfs:isDefinedBy <http://purl.org/ontology/libso> ;
    rdfs:label "Condition"@en, "Nutzungskondition"@de ;
    owl:sameAs service:ServiceLimitation .

lso:CopierBlack
    a rdfs:Class ;
    rdfs:isDefinedBy <http://purl.org/ontology/libso> ;
    rdfs:label "Black and White Copier"@en, "Schwarz-Weiß-Kopierer"@de ;
    rdfs:subClassOf lso:CopierOrScanner .

lso:CopierColor
    a rdfs:Class ;
    rdfs:isDefinedBy <http://purl.org/ontology/libso> ;
    rdfs:label "Color Copier"@en, "Farbkopierer"@de ;
    rdfs:subClassOf lso:CopierOrScanner .

lso:CopierOrScanner
    a rdfs:Class ;
    rdfs:comment "A service provided to enable users making personal copies or scans of documents." ;
    rdfs:isDefinedBy <http://purl.org/ontology/libso> ;
    rdfs:label "Copier or Scanner"@en, "Kopierer oder Scanner"@de ;
    rdfs:subClassOf lso:LocalWork .

lso:Database
    a rdfs:Class ;
    rdfs:isDefinedBy <http://purl.org/ontology/libso> ;
    rdfs:label "Database"@en, "Datenbank"@de ;
    rdfs:subClassOf lso:WebBasedUsage .

lso:ExternalAccess
    a lso:Licence ;
    rdfs:Label "External Access for registered Users"@en, "Externer Zugang für angemeldete Nutzer"@de ;
    rdfs:isDefinedBy <http://purl.org/ontology/libso> .

lso:Free
    a lso:Licence ;
    rdfs:Label "Free Online Access"@en, "Frei im Web verfügbar"@de ;
    rdfs:isDefinedBy <http://purl.org/ontology/libso> .

lso:GroupWorkSpace
    a rdfs:Class ;
    rdfs:comment "A service to provide working space for groups of users." ;
    rdfs:isDefinedBy <http://purl.org/ontology/libso> ;
    rdfs:label "Group Work Room"@en, "Gruppenarbeitsraum"@de ;
    rdfs:subClassOf lso:LocalWork .

lso:IndividualWorkSpace
    a rdfs:Class ;
    rdfs:comment "A service to provide the opportunity for individual work for a single user." ;
    rdfs:isDefinedBy <http://purl.org/ontology/libso> ;
    rdfs:label "Einzelarbeitsplatz"@de, "Individual Work Space"@en ;
    rdfs:subClassOf lso:LocalWork .

lso:InformationCounter
    a rdfs:Class ;
    rdfs:comment "A service provided to inform the library users at a service counter." ;
    rdfs:isDefinedBy <http://purl.org/ontology/libso> ;
    rdfs:label "Information Counter"@en, "Informationstheke"@de ;
    rdfs:subClassOf lso:LocalInformation .

lso:LibraryService
    a:role "abstract" ;
    a rdfs:Class ;
    rdfs:comment "A kind of service provided by a library or a related Institution." ;
    rdfs:isDefinedBy <http://purl.org/ontology/libso> ;
    rdfs:label "Bibliotheksdienstleistung"@de, "Library Service"@en ;
    rdfs:subClassOf service:Service .

lso:LibraryTour
    a rdfs:Class ;
    rdfs:comment "A service provided to guide the users through the library building and to show them the potential uses." ;
    rdfs:isDefinedBy <http://purl.org/ontology/libso> ;
    rdfs:label "Bibliotheksführung"@de, "Library Tour"@en ;
    rdfs:subClassOf lso:LocalInformation .

lso:Licence
    a rdfs:Class ;
    rdfs:comment "class defines conditions for access to databases given by licenses." ;
    rdfs:isDefinedBy <http://purl.org/ontology/libso> ;
    rdfs:label "Licence"@en, "Lizenz"@de ;
    rdfs:subClassOf lso:Condition .

lso:Local
    a rdfs:Class ;
    rdfs:comment "A kind of service that is offered on site at the library." ;
    rdfs:isDefinedBy <http://purl.org/ontology/libso> ;
    rdfs:label "Local Service"@en, "Lokale Dienstleistung"@de ;
    rdfs:subClassOf lso:LibraryService .

lso:LocalInformation
    a rdfs:Class ;
    rdfs:comment "A kind of service provided to inform the library users on site in the library." ;
    rdfs:isDefinedBy <http://purl.org/ontology/libso> ;
    rdfs:label "Local Information Service"@en, "Lokale Informationsvermittlung"@de ;
    rdfs:subClassOf lso:Local .

lso:LocalUsage
    a rdfs:Class ;
    rdfs:comment "A kind of service provided to take use of the library’s media collection." ;
    rdfs:isDefinedBy <http://purl.org/ontology/libso> ;
    rdfs:label "Local Usage Service"@en, "Lokale Bestandsbenutzung"@de ;
    rdfs:subClassOf lso:Local ;
    owl:sameAs dso:documentService .

lso:LocalWork
    a rdfs:Class ;
    rdfs:comment "A service for providing working space and opportunities to the users." ;
    rdfs:isDefinedBy <http://purl.org/ontology/libso> ;
    rdfs:label "Local Work"@en, "Lokales Arbeiten"@de ;
    rdfs:subClassOf lso:Local .

lso:NationalLicence
    a lso:Licence ;
    rdfs:Label "National Licence"@en, "Nationallizenz"@de ;
    rdfs:isDefinedBy <http://purl.org/ontology/libso> .

lso:OnlineInformation
    a rdfs:Class ;
    rdfs:comment "a kind of online service provided to inform the users on the web via chat or email etc." ;
    rdfs:isDefinedBy <http://purl.org/ontology/libso> ;
    rdfs:label "Internetbasierter Auskunftsdienst"@de, "Online Information"@en ;
    rdfs:subClassOf lso:WebBasedInformation .

lso:PCWorkStation
    a rdfs:Class ;
    rdfs:comment "A service to provide the opportunity to do work on a PC." ;
    rdfs:isDefinedBy <http://purl.org/ontology/libso> ;
    rdfs:label "PC Work Station"@en, "PC-Arbeitsplatz"@de ;
    rdfs:subClassOf lso:LocalWork .

lso:POSBuilding
    a rdfs:Class ;
    rdfs:comment "defines a building as a physical site where a local service is available." ;
    rdfs:isDefinedBy <http://purl.org/ontology/libso> ;
    rdfs:label "Building as Point Of Service"@en, "Gebäude als Servicepunkt"@de ;
    rdfs:subClassOf lso:PointOfService, org:OrganizationalUnit .

lso:POSDepartment
    a rdfs:Class ;
    rdfs:comment "defines a department as a physical site where a local service is available." ;
    rdfs:isDefinedBy <http://purl.org/ontology/libso> ;
    rdfs:label "Abteilung als Servicepunkt"@de, "Department as Point Of Service"@en ;
    rdfs:subClassOf lso:PointOfService, org:OrganizationalUnit .

lso:POSUnit
    a rdfs:Class ;
    rdfs:comment "defines an organizational unit as a physical site where a local service is available." ;
    rdfs:isDefinedBy <http://purl.org/ontology/libso> ;
    rdfs:label "Organizational Unit as Point Of Service"@en, "Teilorganisation als Servicepunkt"@de ;
    rdfs:subClassOf lso:PointOfService, org:OrganizationalUnit .

lso:PayPerUse
    a lso:Licence ;
    rdfs:Label "Kostenpflichtiges Angebot"@de, "Paid Offer"@en ;
    rdfs:isDefinedBy <http://purl.org/ontology/libso> .

lso:PhotoService
    a rdfs:Class ;
    rdfs:comment "a service provided to generate photographs for the users." ;
    rdfs:isDefinedBy <http://purl.org/ontology/libso> ;
    rdfs:label "Fotodienst"@de, "Photo Service"@en ;
    rdfs:subClassOf lso:LocalWork .

lso:PointOfService
    a rdfs:Class ;
    rdfs:comment "defines a physical site where a local service is available." ;
    rdfs:isDefinedBy <http://purl.org/ontology/libso> ;
    rdfs:label "Point of Service"@en, "Servicepunkt"@de ;
    rdfs:subClassOf org:OrganizationalUnit .

lso:Recommendation
    a rdfs:Class ;
    rdfs:isDefinedBy <http://purl.org/ontology/libso> ;
    rdfs:label "Anschaffungsempfehlung"@en, "Purchase Recommendation"@en ;
    rdfs:subClassOf lso:WebBasedUsage .

lso:Registration
    a rdfs:Class ;
    rdfs:comment "An action to register a person as a library user and inform it about usage opportunities and conditions." ;
    rdfs:isDefinedBy <http://purl.org/ontology/libso> ;
    rdfs:label "Nutzeranmeldung"@de, "User Registration"@en ;
    rdfs:subClassOf lso:LocalInformation .

lso:ResearchStation
    a rdfs:Class ;
    rdfs:comment "A PC-Station provided for research within the library’s media collection." ;
    rdfs:isDefinedBy <http://purl.org/ontology/libso> ;
    rdfs:label "Rechercheplatz"@de, "Research Station"@en ;
    rdfs:subClassOf lso:LocalUsage .

lso:SingleUser
    a lso:Licence ;
    rdfs:Label "Einzelplatzversion"@de, "Sinlge User Version"@en ;
    rdfs:isDefinedBy <http://purl.org/ontology/libso> .

lso:SubService
    a rdfs:Class ;
    rdfs:comment "Defines a single component of a higher-level service" ;
    rdfs:isDefinedBy <http://purl.org/ontology/libso> ;
    rdfs:label "Dienstleistungsbestandteil"@de, "Service Component"@en ;
    rdfs:subClassOf lso:LibraryService .

lso:UserTraining
    a rdfs:Class ;
    rdfs:comment "A service provided to train the users in research and use of the library’s media collection." ;
    rdfs:isDefinedBy <http://purl.org/ontology/libso> ;
    rdfs:label "Nutzerschulung"@de, "User Training"@en ;
    rdfs:subClassOf lso:LocalInformation .

lso:WebBased
    a rdfs:Class ;
    rdfs:comment "A kind of online service provided on the library’s website." ;
    rdfs:isDefinedBy <http://purl.org/ontology/libso> ;
    rdfs:label "Internetbasierte Dienstleistung"@de, "Web Based Service"@en ;
    rdfs:subClassOf lso:LibraryService .

lso:WebBasedInformation
    a rdfs:Class ;
    rdfs:comment "a kind of online service provided to inform the users on the web." ;
    rdfs:isDefinedBy <http://purl.org/ontology/libso> ;
    rdfs:label "Internetbasierter Auskunftsdienst"@de, "Web Based Information Service"@en ;
    rdfs:subClassOf lso:WebBased .

lso:WebBasedUsage
    a rdfs:Class ;
    rdfs:comment "A kind of online service provided to gain access to parts of the media collection on the web." ;
    rdfs:isDefinedBy <http://purl.org/ontology/libso> ;
    rdfs:label "Internetbasierte Bestandsbenutzung"@de, "Web Based Usage Service"@en ;
    rdfs:subClassOf lso:WebBased .

lso:floor
    a rdfs:Property ;
    rdfs:domain lso:POSDepartment ;
    rdfs:isDefinedBy <http://purl.org/ontology/libso> ;
    rdfs:label "Etage oder Ebene"@de, "floor"@en ;
    rdfs:range rdfs:Literal .

lso:hasAccessURL
    a rdf:Property ;
    rdfs:domain lso:WebBased ;
    rdfs:isDefinedBy <http://purl.org/ontology/libso> ;
    rdfs:label "Zugang über URL"@de, "has access URL"@en ;
    rdfs:range rdfs:Literal .

lso:hasCondition
    a rdf:Property ;
    rdfs:domain lso:LibraryService ;
    rdfs:isDefinedBy <http://purl.org/ontology/libso> ;
    rdfs:label "Nutzungskonditionen"@de, "has condition"@en ;
    rdfs:range lso:Condition .

lso:hasLicence
    a rdfs:Property ;
    rdfs:domain lso:WebBasedUsage ;
    rdfs:isDefinedBy <http://purl.org/ontology/libso> ;
    rdfs:label "has Licence"@en, "unter Lizenz"@de ;
    rdfs:range lso:Licence .

lso:hasOptionalWebAccess
    a rdf:Property ;
    rdfs:domain lso:Local ;
    rdfs:isDefinedBy <http://purl.org/ontology/libso> ;
    rdfs:label "Alternativer Internetzugang"@de, "has optional web access"@en ;
    rdfs:range lso:WebBased .

lso:hasPeriodTime
    a rdfs:Property ;
    rdfs:domain lso:Condition ;
    rdfs:isDefinedBy <http://purl.org/ontology/libso> ;
    rdfs:label "has Period Time"@en, "zugehörige Frist"@de ;
    rdfs:range rdfs:Literal .

lso:hasPointOfService
    a rdf:Property ;
    rdfs:domain lso:Local ;
    rdfs:isDefinedBy <http://purl.org/ontology/libso> ;
    rdfs:label "has point of service"@en, "verfügbar am Standort"@de ;
    rdfs:range lso:PointOfService .

lso:relatedDocument
    a rdfs:Property ;
    rdfs:domain rdfs:Condition ;
    rdfs:isDefinedBy <http://purl.org/ontology/libso> ;
    rdfs:label "Zugehöriges Dokument"@de, "related Document"@en ;
    rdfs:range rdfs:Literal .

lso:room
    a rdfs:Property ;
    rdfs:domain lso:POSDepartment ;
    rdfs:isDefinedBy <http://purl.org/ontology/libso> ;
    rdfs:label "Zimmernummer"@de, "room number"@en ;
    rdfs:range rdfs:Literal .

lso:staffContact
    a rdfs:Property ;
    rdfs:domain lso:LibraryService ;
    rdfs:isDefinedBy <http://purl.org/ontology/libso> ;
    rdfs:label "Kontakt zum Personal"@de, "staff Contact"@en ;
    rdfs:range vcard:Individual, vcard:Organization .

service:Service
    a owl:Class ;
    rdfs:isDefinedBy <http://purl.org/ontology/service> ;
    rdfs:label "Service"@en ;
    rdfs:seeAlso s:Product, s:Service ;
    rdfs:subClassOf dct:Service, gr:ProductOrService .

service:ServiceProvider
    a rdfs:Class ;
    rdfs:isDefinedBy <http://purl.org/ontology/service> ;
    rdfs:label "ServiceProvider"@en ;
    rdfs:seeAlso dct:agent, gr:BusinessEntity, s:Organization, s:person, foaf:agent .

service:providedBy
    a owl:ObjectProperty ;
    rdfs:domain service:Service ;
    rdfs:isDefinedBy <http://purl.org/ontology/service> ;
    rdfs:label "providedBy"@en ;
    rdfs:range service:ServiceProvider ;
    rdfs:seeAlso s:provider ;
    owl:inverseOf service:provides .

service:provides
    a owl:ObjectProperty ;
    rdfs:domain service:ServiceProvider ;
    rdfs:isDefinedBy <http://purl.org/ontology/service> ;
    rdfs:label "provides"@en ;
    rdfs:range service:Service ;
    owl:inverseOf service:providedBy .

geo:Location
    a rdfs:Class .

geo:lat
    a rdfs:Property ;
    rdfs:domain geo:Location ;
    rdfs:range rdfs:Literal .

geo:location
    a rdfs:Property ;
    rdfs:domain org:Site ;
    rdfs:range geo:Location .

geo:long
    a rdfs:Property ;
    rdfs:domain geo:Location ;
    rdfs:range rdfs:Literal .

vcard:Address
    a owl:Class ;
    rdfs:comment "To specify the components of the delivery address for the object"^^xsd:string ;
    rdfs:isDefinedBy <http://www.w3.org/2006/vcard/ns> ;
    rdfs:label "Address"^^xsd:string .

vcard:Email
    a owl:Class ;
    rdfs:comment """To specify the electronic mail address for communication
        with the object the vCard represents. Use the hasEmail object property."""^^xsd:string ;
    rdfs:isDefinedBy <http://www.w3.org/2006/vcard/ns> ;
    rdfs:label "Email"^^xsd:string ;
    owl:deprecated true .

vcard:Fax
    a owl:Class ;
    rdfs:isDefinedBy <http://www.w3.org/2006/vcard/ns> ;
    rdfs:label "Fax"^^xsd:string ;
    rdfs:subClassOf vcard:TelephoneType .

vcard:Individual
    a owl:Class ;
    rdfs:comment "An object representing a single person or entity"^^xsd:string ;
    rdfs:isDefinedBy <http://www.w3.org/2006/vcard/ns> ;
    rdfs:label "Individual"^^xsd:string ;
    rdfs:subClassOf vcard:Kind ;
    owl:disjointWith vcard:Location, vcard:Organization .

vcard:Organization
    a owl:Class ;
    rdfs:comment """An object representing an organization. An organization
        is a single entity, and might represent a business or government, a department
        or division within a business or government, a club, an association, or the
        like."""^^xsd:string ;
    rdfs:isDefinedBy <http://www.w3.org/2006/vcard/ns> ;
    rdfs:label "Organization"^^xsd:string ;
    rdfs:subClassOf vcard:Kind .

vcard:Voice
    a owl:Class ;
    rdfs:isDefinedBy <http://www.w3.org/2006/vcard/ns> ;
    rdfs:label "Voice"^^xsd:string ;
    rdfs:subClassOf vcard:TelephoneType .

vcard:country-name
    a owl:DatatypeProperty ;
    rdfs:comment "The country name associated with the address of the object" ;
    rdfs:isDefinedBy <http://www.w3.org/2006/vcard/ns> ;
    rdfs:label "country name"^^xsd:string ;
    rdfs:range xsd:string .

vcard:fn
    a owl:DatatypeProperty ;
    rdfs:comment "The formatted text corresponding to the name of the object" ;
    rdfs:isDefinedBy <http://www.w3.org/2006/vcard/ns> ;
    rdfs:label "formatted name"^^xsd:string ;
    rdfs:range xsd:string .

vcard:hasAddress
    a owl:ObjectProperty ;
    rdfs:comment "To specify the components of the delivery address for the object"^^xsd:string ;
    rdfs:isDefinedBy <http://www.w3.org/2006/vcard/ns> ;
    rdfs:label "has address"^^xsd:string ;
    rdfs:range vcard:Address .

vcard:hasEmail
    a owl:ObjectProperty ;
    rdfs:comment "To specify the electronic mail address for communication with the object"^^xsd:string ;
    rdfs:isDefinedBy <http://www.w3.org/2006/vcard/ns> ;
    rdfs:label "has email"^^xsd:string ;
    rdfs:range vcard:Email .

vcard:hasTelephone
    a owl:ObjectProperty ;
    rdfs:comment "To specify the telephone number for telephony communication with the object"^^xsd:string ;
    rdfs:isDefinedBy <http://www.w3.org/2006/vcard/ns> ;
    rdfs:label "has telephone"^^xsd:string ;
    owl:equivalentProperty vcard:tel .

vcard:hasValue
    a owl:ObjectProperty ;
    rdfs:comment "Used to indicate the resource value of an object property that requires property parameters"^^xsd:string ;
    rdfs:isDefinedBy <http://www.w3.org/2006/vcard/ns> ;
    rdfs:label "has value"@en .

vcard:locality
    a owl:DatatypeProperty ;
    rdfs:comment "The locality (e.g. city or town) associated with the address of the object" ;
    rdfs:isDefinedBy <http://www.w3.org/2006/vcard/ns> ;
    rdfs:label "locality"^^xsd:string ;
    rdfs:range xsd:string .

vcard:organization-name
    a owl:DatatypeProperty ;
    rdfs:comment "To specify the organizational name associated with the object" ;
    rdfs:isDefinedBy <http://www.w3.org/2006/vcard/ns> ;
    rdfs:label "organization name"^^xsd:string ;
    rdfs:range xsd:string .

vcard:postal-code
    a owl:DatatypeProperty ;
    rdfs:comment "The postal code associated with the address of the object" ;
    rdfs:isDefinedBy <http://www.w3.org/2006/vcard/ns> ;
    rdfs:label "postal code"^^xsd:string ;
    rdfs:range xsd:string .

vcard:street-address
    a owl:DatatypeProperty ;
    rdfs:comment "The street address associated with the address of the object" ;
    rdfs:isDefinedBy <http://www.w3.org/2006/vcard/ns> ;
    rdfs:label "street address"^^xsd:string ;
    rdfs:range xsd:string .

org:Organization
    a rdfs:Class, owl:Class ;
    rdfs:comment """Represents a collection of people organized together into a
        community or other social, commercial or political structure. The group has
        some common purpose or reason for existence which goes beyond the set of
        people belonging to it and can act as an Agent. Organizations are often 
        decomposable into hierarchical structures. It is recommended that SKOS lexical labels
        should be used to label the Organization. In particular `skos:prefLabel` for
        the primary (possibly legally recognized name), `skos:altLabel` for alternative
        names (trading names, colloquial names) and `skos:notation` to denote a
        code from a code list. Alternative names: _Collective_ _Body_ _Org_ _Group_"""@en ;
    rdfs:isDefinedBy <http://www.w3.org/ns/org> ;
    rdfs:label "Organization"@en ;
    rdfs:subClassOf foaf:Agent ;
    owl:equivalentClass foaf:Organization ;
    owl:hasKey (org:identifier
    ) .

org:OrganizationalUnit
    a rdfs:Class, owl:Class ;
    rdfs:comment """An Organization such as a University Support Unit which is
        part of some larger FormalOrganization and only has full recognition within
        the context of that FormalOrganization, it is not a Legal Entity in its own
        right. Units can be large and complex containing other Units and even
        FormalOrganizations. Alternative names: _OU_ _Unit_ _Department_"""@en ;
    rdfs:isDefinedBy <http://www.w3.org/ns/org> ;
    rdfs:label "OrganizationalUnit"@en ;
    rdfs:subClassOf org:Organization .

org:Site
    a rdfs:Class, owl:Class ;
    rdfs:comment """An office or other premise at which the organization is
        located. Many organizations are spread across multiple sites and many sites will
        host multiple locations. In most cases a Site will be a physical location.
        However, we don't exclude the possibility of non-physical sites such as a
        virtual office with an associated post box and phone reception service. 
        Extensions may provide subclasses to denote particular types of site."""@en ;
    rdfs:isDefinedBy <http://www.w3.org/ns/org> ;
    rdfs:label "Site"@en .

org:hasSite
    a rdf:Property, owl:ObjectProperty ;
    rdfs:comment """Indicates a site at which the Organization has some presence
    even if only indirect (e.g. virtual office or a professional service which is
    acting as the registered address for a company). Inverse of `org:siteOf`."""@en ;
    rdfs:domain org:Organization ;
    rdfs:isDefinedBy <http://www.w3.org/ns/org> ;
    rdfs:label "has site"@en ;
    rdfs:range org:Site .

org:hasUnit
    a rdf:Property, owl:ObjectProperty ;
    rdfs:comment """Indicates a unit which is part of this Organization, e.g. a
        Department within a larger FormalOrganization. Inverse of `org:unitOf`."""@en ;
    rdfs:domain org:FormalOrganization ;
    rdfs:isDefinedBy <http://www.w3.org/ns/org> ;
    rdfs:label "has Unit"@en ;
    rdfs:range org:OrganizationalUnit ;
    rdfs:subPropertyOf org:hasSubOrganization .

org:unitOf
    a rdf:Property, owl:ObjectProperty ;
    rdfs:comment """Indicates an Organization of which this Unit is a part, e.g.
    a Department within a larger FormalOrganization. This is the inverse of
    `org:hasUnit`."""@en ;
    rdfs:domain org:OrganizationalUnit ;
    rdfs:isDefinedBy <http://www.w3.org/ns/org> ;
    rdfs:label "unit Of"@en ;
    rdfs:range org:FormalOrganization ;
    rdfs:subPropertyOf org:subOrganizationOf .

